Updated to newest version of VST.
Requires Coq 8.10.

atomics/general_atomics.v
@@ -1,4 +1,4 @@
-Require Import VST.veric.rmaps.
+ Require Import VST.veric.rmaps.
 Require Import VST.veric.compcert_rmaps.
 Require Import VST.progs.ghosts.
 Require Import VST.progs.conclib.
@@ -28,6 +28,16 @@ Set Bullet Behavior "Strict Subproofs".
    since we can't insert it into the definition of semax? Well, iGPS still uses it in the RA atomic
    rules, so maybe it's still useful. *)
 
+(* up *)
+Lemma later_nonexpansive : forall n P, approx n (|> P) = approx n (|> approx n P).
+Proof.
+  intros.
+  destruct n; [rewrite !approx_0; auto|].
+  rewrite !approx_later; f_equal.
+  change (approx n (approx (S n) P)) with ((approx n oo approx (S n)) P).
+  rewrite -> approx_oo_approx'; auto.
+Qed.
+
 Section atomics.
 
 Context {CS : compspecs} {inv_names : invG}.
@@ -36,10 +46,226 @@ Section atomicity.
 
 (* The logical atomicity of Iris. *)
 (* We use the cored predicate to mimic Iris's persistent modality. *)
-Definition atomic_shift {A B} (a : A -> mpred) Ei Eo (b : A -> B -> mpred) (Q : B -> mpred) :=
-  EX P : mpred, |> P * ((|> P -* |={Eo,Ei}=> (EX x : A, a x *
+Definition ashift {A B} P (a : A -> mpred) Ei Eo (b : A -> B -> mpred) (Q : B -> mpred) :=
+  ((|> P -* |={Eo,Ei}=> (EX x : A, a x *
     ((a x -* |={Ei,Eo}=> |> P) &&
-     ALL y : B, b x y -* |={Ei,Eo}=> Q y))) && cored)%I.
+     ALL y : B, b x y -* |={Ei,Eo}=> Q y))))%I.
+
+Definition atomic_shift {A B} (a : A -> mpred) Ei Eo (b : A -> B -> mpred) (Q : B -> mpred) :=
+  EX P : mpred, |> P * (ashift P a Ei Eo b Q && cored).
+
+(* up *)
+Lemma allp_nonexpansive : forall {A} n P, approx n (ALL y : A, P y) = approx n (ALL y, approx n (P y)).
+Proof.
+  intros.
+  apply predicates_hered.pred_ext; intros ? [? Hall]; split; auto; intro; simpl in *.
+  - split; auto.
+  - apply Hall.
+Qed.
+
+Lemma ashift_nonexpansive : forall {A B} P n a Ei Eo (b : A -> B -> mpred) Q,
+  approx n (ashift P a Ei Eo b Q) =
+  approx n (ashift P (fun x => approx n (a x)) Ei Eo (fun x y => approx n (b x y)) (fun y => approx n (Q y))).
+Proof.
+  intros; unfold ashift.
+  setoid_rewrite fview_shift_nonexpansive; f_equal; f_equal; f_equal.
+  rewrite !approx_exp; f_equal; extensionality.
+  rewrite -> !approx_sepcon, !approx_andp, !approx_idem; f_equal; auto.
+  f_equal.
+  * setoid_rewrite fview_shift_nonexpansive; rewrite !approx_idem; f_equal; f_equal; auto.
+  * rewrite allp_nonexpansive; setoid_rewrite allp_nonexpansive at 2; f_equal; f_equal; extensionality.
+    setoid_rewrite fview_shift_nonexpansive; rewrite !approx_idem; auto.
+Qed.
+
+Lemma atomic_shift_nonexpansive : forall {A B} n a Ei Eo (b : A -> B -> mpred) Q,
+  approx n (atomic_shift a Ei Eo b Q) =
+  approx n (atomic_shift (fun x => approx n (a x)) Ei Eo (fun x y => approx n (b x y)) (fun y => approx n (Q y))).
+Proof.
+  intros; unfold atomic_shift.
+  rewrite !approx_exp; f_equal; extensionality.
+  rewrite !approx_sepcon !approx_andp ashift_nonexpansive; auto.
+Qed.
+
+(* up *)
+Lemma cored_sepcon: forall P Q, (P && cored) * (Q && cored) |-- (P * Q) && cored.
+Proof.
+  intros.
+  apply andp_right.
+  + apply sepcon_derives; apply andp_left1; auto.
+  + eapply derives_trans; [apply sepcon_derives; apply andp_left2, derives_refl|].
+      rewrite <- cored_duplicable; auto.
+Qed.
+
+Lemma cored_dup_gen : forall P, P |-- cored -> P |-- P * P.
+Proof.
+  intros.
+  erewrite (add_andp P) by apply H; apply cored_dup.
+Qed.
+
+Lemma atomic_shift_derives_frame_cored : forall {A A' B B'} (a : A -> mpred) (a' : A' -> mpred) Ei Eo
+  (b : A -> B -> mpred) (b' : A' -> B' -> mpred) (Q : B -> mpred) (Q' : B' -> mpred) F R
+  (HF : F |-- cored)
+  (Ha : (forall x, a x * F * |>R |-- |={Ei}=> EX x' : A', a' x' *
+    ((a' x' -* |={Ei}=> a x * |>R) && ALL y' : _, b' x' y' -* |={Ei}=> EX y : _, b x y * (Q y -* |={Eo}=> Q' y')))%I),
+  atomic_shift a Ei Eo b Q * F * |>R |-- atomic_shift a' Ei Eo b' Q'.
+Proof.
+  intros; unfold atomic_shift, ashift.
+  Intros P; Exists (P * R); rewrite later_sepcon; cancel.
+  erewrite (add_andp F) by apply HF.
+  sep_apply cored_sepcon.
+  apply andp_derives; auto.
+  iIntros "[H F] [P R]"; iMod ("H" with "P") as (x) "[a H]".
+  iMod (Ha with "[$a $F $R]") as (x') "[? Hrest]"; iExists x'; iFrame.
+  iIntros "!>"; iSplit.
+  - iIntros "a".
+    iDestruct "Hrest" as "[Hrest _]".
+    iMod ("Hrest" with "a") as "[? $]"; iApply "H"; auto.
+  - iIntros (y') "b".
+    iDestruct "Hrest" as "[_ Hb]".
+    iMod ("Hb" $! y' with "b") as (y) "[b HQ]".
+    iMod ("H" with "b").
+    iApply "HQ"; auto.
+Qed.
+
+Lemma atomic_shift_derives_frame : forall {A A' B B'} (a : A -> mpred) (a' : A' -> mpred) Ei Eo
+  (b : A -> B -> mpred) (b' : A' -> B' -> mpred) (Q : B -> mpred) (Q' : B' -> mpred) R
+  (Ha : (forall x, a x * |>R |-- |={Ei}=> EX x' : A', a' x' *
+    ((a' x' -* |={Ei}=> a x * |>R) && ALL y' : _, b' x' y' -* |={Ei}=> EX y : _, b x y * (Q y -* |={Eo}=> Q' y')))%I),
+  atomic_shift a Ei Eo b Q * |>R |-- atomic_shift a' Ei Eo b' Q'.
+Proof.
+  intros; unfold atomic_shift, ashift.
+  Intros P; Exists (P * R); rewrite later_sepcon; cancel.
+  apply andp_derives; auto.
+  iIntros "H [P R]"; iMod ("H" with "P") as (x) "[a H]".
+  iMod (Ha with "[$a $R]") as (x') "[? Hrest]"; iExists x'; iFrame.
+  iIntros "!>"; iSplit.
+  - iIntros "a".
+    iMod ("Hrest" with "a") as "[? $]"; iApply "H"; auto.
+  - iIntros (y') "b".
+    iDestruct "Hrest" as "[_ Hb]".
+    iMod ("Hb" $! y' with "b") as (y) "[b HQ]".
+    iMod ("H" with "b").
+    iApply "HQ"; auto.
+Qed.
+
+Lemma ashift_derives : forall {A A' B B'} P (a : A -> mpred) (a' : A' -> mpred) Ei Eo
+  (b : A -> B -> mpred) (b' : A' -> B' -> mpred) (Q : B -> mpred) (Q' : B' -> mpred)
+  (Ha : (forall x, a x  |-- |={Ei}=> EX x' : A', a' x' *
+    (((a' x' * (ashift P a Ei Eo b Q && cored)) -* |={Ei}=> a x) &&
+     ALL y' : _, (b' x' y' * (ashift P a Ei Eo b Q && cored)) -* |={Ei}=> EX y : _, b x y * (Q y -* |={Eo}=> Q' y')))%I),
+  ashift P a Ei Eo b Q && cored |-- ashift P a' Ei Eo b' Q' && cored.
+Proof.
+  intros.
+  sep_apply cored_dup_cored.
+  apply andp_derives; auto.
+  unfold ashift at 1 3.
+  iIntros "[H AS] P"; iMod ("H" with "P") as (x) "[a H]".
+  iMod (Ha with "a") as (x') "[? Hrest]"; iExists x'; iFrame.
+  iIntros "!>"; iSplit.
+  - iIntros "a".
+    iDestruct "Hrest" as "[Hrest _]".
+    iMod ("Hrest" with "[$a $AS]") as "a"; iApply "H"; auto.
+  - iIntros (y') "b".
+    iDestruct "Hrest" as "[_ Hb]".
+    iMod ("Hb" $! y' with "[$b $AS]") as (y) "[b HQ]".
+    iMod ("H" with "b").
+    iApply "HQ"; auto.
+Qed.
+
+Lemma atomic_shift_derives : forall {A A' B B'} (a : A -> mpred) (a' : A' -> mpred) Ei Eo
+  (b : A -> B -> mpred) (b' : A' -> B' -> mpred) (Q : B -> mpred) (Q' : B' -> mpred)
+  (Ha : (forall x, a x  |-- |={Ei}=> EX x' : A', a' x' *
+    ((a' x' -* |={Ei}=> a x) && ALL y' : _, b' x' y' -* |={Ei}=> EX y : _, b x y * (Q y -* |={Eo}=> Q' y')))%I),
+  atomic_shift a Ei Eo b Q |-- atomic_shift a' Ei Eo b' Q'.
+Proof.
+  intros; eapply derives_trans, atomic_shift_derives_frame.
+  { rewrite <- sepcon_emp at 1; apply sepcon_derives; [apply derives_refl | apply now_later]. }
+  iIntros (x) "[a >_]".
+  iMod (Ha with "a") as (x') "[? H]".
+  iExists x'; iFrame; iIntros "!>"; iSplit.
+  - iIntros "a"; iMod ("H" with "a") as "$"; auto.
+  - iDestruct "H" as "[_ H]"; auto.
+Qed.
+
+Lemma atomic_shift_derives_cored : forall {A A' B B'} (a : A -> mpred) (a' : A' -> mpred) Ei Eo
+  (b : A -> B -> mpred) (b' : A' -> B' -> mpred) (Q : B -> mpred) (Q' : B' -> mpred) F
+  (HF : F |-- cored)
+  (Ha : (forall x, a x * F |-- |={Ei}=> EX x' : A', a' x' *
+    ((a' x' -* |={Ei}=> a x) && ALL y' : _, b' x' y' -* |={Ei}=> EX y : _, b x y * (Q y -* |={Eo}=> Q' y')))%I),
+  atomic_shift a Ei Eo b Q * F |-- atomic_shift a' Ei Eo b' Q'.
+Proof.
+  intros; eapply derives_trans, atomic_shift_derives_frame_cored; eauto.
+  { rewrite <- sepcon_emp at 1; apply sepcon_derives; [apply derives_refl | apply now_later]. }
+  iIntros (x) "[a >_]".
+  iMod (Ha with "a") as (x') "[? H]".
+  iExists x'; iFrame; iIntros "!>"; iSplit.
+  - iIntros "a"; iMod ("H" with "a") as "$"; auto.
+  - iDestruct "H" as "[_ H]"; auto.
+Qed.
+
+Lemma atomic_shift_derives' : forall {A A' B} (a : A -> mpred) (a' : A' -> mpred) Ei Eo
+  (b : A -> B -> mpred) (b' : A' -> B -> mpred) (Q : B -> mpred)
+  (Ha : (forall x, a x |-- |={Ei}=> EX x' : A', a' x' *
+    ((a' x' -* |={Ei}=> a x) && ALL y : _, b' x' y -* |={Ei}=> b x y))%I),
+  atomic_shift a Ei Eo b Q |-- atomic_shift a' Ei Eo b' Q.
+Proof.
+  intros; apply atomic_shift_derives.
+  iIntros (x) "a"; iMod (Ha with "a") as (x') "[a H]".
+  iExists x'; iFrame.
+  iIntros "!>"; iSplit.
+  - iIntros "a"; iMod ("H" with "a") as "$"; auto.
+  - iIntros (y) "b"; iExists y.
+    iDestruct "H" as "[_ H]".
+    iMod ("H" with "b") as "$".
+    iIntros "!> $"; auto.
+Qed.
+
+Lemma atomic_shift_derives'_cored : forall {A A' B} (a : A -> mpred) (a' : A' -> mpred) Ei Eo
+  (b : A -> B -> mpred) (b' : A' -> B -> mpred) (Q : B -> mpred) F
+  (HF : F |-- cored)
+  (Ha : (forall x, a x * F |-- |={Ei}=> EX x' : A', a' x' *
+    ((a' x' -* |={Ei}=> a x) && ALL y : _, b' x' y -* |={Ei}=> b x y))%I),
+  atomic_shift a Ei Eo b Q * F |-- atomic_shift a' Ei Eo b' Q.
+Proof.
+  intros; apply atomic_shift_derives_cored; auto.
+  iIntros (x) "a"; iMod (Ha with "a") as (x') "[a H]".
+  iExists x'; iFrame.
+  iIntros "!>"; iSplit.
+  - iIntros "a"; iMod ("H" with "a") as "$"; auto.
+  - iIntros (y) "b"; iExists y.
+    iDestruct "H" as "[_ H]".
+    iMod ("H" with "b") as "$".
+    iIntros "!> $"; auto.
+Qed.
+
+Lemma atomic_shift_derives_simple : forall {A B} (a a' : A -> mpred) Ei Eo (b b' : A -> B -> mpred) (Q : B -> mpred)
+  (Ha1 : (forall x, a x |-- |={Ei}=> a' x)%I)
+  (Ha2 : (forall x, a' x |-- |={Ei}=> a x)%I)
+  (Hb : (forall x y, b' x y |-- |={Ei}=> b x y)%I),
+  atomic_shift a Ei Eo b Q |-- atomic_shift a' Ei Eo b' Q.
+Proof.
+  intros; apply atomic_shift_derives'; intros.
+  iIntros "a"; iExists x; iMod (Ha1 with "a") as "$".
+  iIntros "!>"; iSplit.
+  - iApply Ha2.
+  - iIntros (?); iApply Hb.
+Qed.
+
+Lemma atomic_shift_exists : forall {A B} a Ei Eo (b : A -> B -> mpred) Q,
+  atomic_shift (fun (_ : unit) => EX x : A, a x) Ei Eo (fun (_ : unit) => EX x : A, b x) Q |-- atomic_shift a Ei Eo b Q.
+Proof.
+  intros; unfold atomic_shift.
+  Intros P; Exists P; cancel.
+  unfold ashift.
+  apply andp_derives; auto.
+  iIntros "H P"; iMod ("H" with "P") as (_) "[a H]".
+  iDestruct "a" as (x) "a"; iExists x; iFrame.
+  iIntros "!>"; iSplit.
+  - iIntros "a"; iApply "H".
+    iExists x; auto.
+  - iIntros (y) "b"; iApply "H".
+    simpl; iExists x; auto.
+Qed.
 
 End atomicity.
 
@@ -48,12 +274,12 @@ End atomics.
 Definition atomic_spec_type W T := ProdType (ProdType W (ArrowType (ConstType T) Mpred)) (ConstType invG).
 
 Definition super_non_expansive_a {A W} (a : forall ts : list Type, functors.MixVariantFunctor._functor
-  (dependent_type_functor_rec ts W) (predicates_hered.pred rmap) -> A -> predicates_hered.pred rmap) :=
+  (dependent_type_functor_rec ts W) (predicates_hered.pred rmap) -> A ts -> predicates_hered.pred rmap) :=
   forall n ts w x, approx n (a ts w x) =
   approx n (a ts (functors.MixVariantFunctor.fmap (dependent_type_functor_rec ts W) (approx n) (approx n) w) x).
 
 Definition super_non_expansive_b {A B W} (b : forall ts : list Type, functors.MixVariantFunctor._functor
-  (dependent_type_functor_rec ts W) (predicates_hered.pred rmap) -> A -> B -> predicates_hered.pred rmap) :=
+  (dependent_type_functor_rec ts W) (predicates_hered.pred rmap) -> A ts -> B ts -> predicates_hered.pred rmap) :=
   forall n ts w x y, approx n (b ts w x y) =
   approx n (b ts (functors.MixVariantFunctor.fmap (dependent_type_functor_rec ts W) (approx n) (approx n) w) x y).
 
@@ -61,7 +287,7 @@ Definition super_non_expansive_la {W} la := forall n ts w rho,
   Forall (fun l => approx n (!! locald_denote (l ts w) rho) = approx n (!! locald_denote (l ts
     (functors.MixVariantFunctor.fmap (dependent_type_functor_rec ts W) (approx n) (approx n) w)) rho)) la.
 
-Definition super_non_expansive_lb {B W} lb := forall n ts w (v : B) rho,
+Definition super_non_expansive_lb {B W} lb := forall n ts w (v : B ts) rho,
   Forall (fun l => approx n (!! locald_denote (l ts w v) rho) = approx n (!! locald_denote (l ts
     (functors.MixVariantFunctor.fmap (dependent_type_functor_rec ts W) (approx n) (approx n) w) v) rho)) lb.
 
@@ -79,6 +305,7 @@ Import List.
      PROP () (LOCALx (map (fun l => l ts w v) lb)
      (SEP (Q v)))) _ _).*)
 
+
 Lemma atomic_spec_nonexpansive_pre' : forall {A T} {t : Inhabitant T} W P L R S2 Ei Eo SQ
   (HP : Forall (fun x => super_non_expansive (fun ts w _ => !! (x ts w))) P)
   (HL : Forall (fun x => super_non_expansive (fun ts w rho => !! (locald_denote (x ts w) rho))) L)
@@ -89,12 +316,12 @@ Lemma atomic_spec_nonexpansive_pre' : forall {A T} {t : Inhabitant T} W P L R S2
   (fun ts (_a : functors.MixVariantFunctor._functor (dependent_type_functor_rec ts W) mpred * (T -> mpred) * invG) =>
     let '(w, Q, inv_names) := _a in
     PROPx (map (fun P => P ts w) P) (LOCALx (map (fun L => L ts w) L)
-     (SEPx (atomic_shift(A := A)(inv_names := inv_names) (S2 ts w) Ei Eo (SQ ts w) Q :: map (fun R => R ts w) R)))).
+     (SEPx (atomic_shift(A := A ts)(inv_names := inv_names) (S2 ts w) Ei Eo (SQ ts w) Q :: map (fun R => R ts w) R)))).
 Proof.
   intros.
   replace _ with (fun ts (_a : functors.MixVariantFunctor._functor (dependent_type_functor_rec ts W) mpred * (T -> mpred) * invG) rho =>
     PROPx (map (fun P => P ts _a) (map (fun P ts _a => let '(w, _, _) := _a in P ts w) P)) (LOCALx (map (fun P => P ts _a) (map (fun P ts _a => let '(w, _, _) := _a in P ts w) L))
-     (SEPx (map (fun R => R ts _a) ((fun ts _a => let '(w, Q, inv_names) := _a in atomic_shift(A := A)(inv_names := inv_names) (S2 ts w) Ei Eo (SQ ts w) Q) ::
+     (SEPx (map (fun R => R ts _a) ((fun ts _a => let '(w, Q, inv_names) := _a in atomic_shift(A := A ts)(inv_names := inv_names) (S2 ts w) Ei Eo (SQ ts w) Q) ::
         map (fun R ts _a => let '(w, _, _) := _a in R ts w) R)))) rho).
   apply PROP_LOCAL_SEP_super_non_expansive.
   - rewrite Forall_map.
@@ -104,18 +331,10 @@ Proof.
     eapply Forall_impl, HL; simpl; intros.
     intros ?? ((?, ?), ?) ?; simpl; auto.
   - constructor.
-    + intros ?? ((?, ?), ?) ?.
-      unfold atomic_shift; simpl.
-      rewrite !approx_exp; f_equal; extensionality.
-      rewrite -> !approx_sepcon, !approx_andp; f_equal; f_equal.
-      setoid_rewrite fview_shift_nonexpansive; f_equal; f_equal; f_equal.
-      rewrite !approx_exp; f_equal; extensionality.
-      rewrite -> !approx_sepcon, !approx_andp; f_equal; auto.
-      f_equal.
-      * setoid_rewrite fview_shift_nonexpansive; f_equal; f_equal; auto.
-      * rewrite -> !approx_allp by auto; f_equal; extensionality.
-        setoid_rewrite fview_shift_nonexpansive; f_equal; f_equal; auto.
-        rewrite approx_idem; auto.
+    + intros ?? ((?, ?), ?) ?; simpl.
+      rewrite -> atomic_shift_nonexpansive by auto; setoid_rewrite atomic_shift_nonexpansive at 2; auto.
+      f_equal; f_equal; repeat extensionality; auto.
+      rewrite approx_idem; auto.
     + rewrite Forall_map.
       eapply Forall_impl, HR; simpl; intros.
       intros ?? ((?, ?), ?) ?; simpl; auto.
@@ -136,12 +355,12 @@ Lemma atomic_spec_nonexpansive_pre0 : forall {A} W P L R S2 Ei Eo SQ
   (fun ts (_a : functors.MixVariantFunctor._functor (dependent_type_functor_rec ts W) mpred * mpred * invG) =>
     let '(w, Q, inv_names) := _a in
     PROPx (map (fun P => P ts w) P) (LOCALx (map (fun L => L ts w) L)
-     (SEPx (atomic_shift(A := A)(B := unit)(inv_names := inv_names) (S2 ts w) Ei Eo (SQ ts w) (fun _ => Q) :: map (fun R => R ts w) R)))).
+     (SEPx (atomic_shift(A := A ts)(B := unit)(inv_names := inv_names) (S2 ts w) Ei Eo (SQ ts w) (fun _ => Q) :: map (fun R => R ts w) R)))).
 Proof.
   intros.
   replace _ with (fun ts (_a : functors.MixVariantFunctor._functor (dependent_type_functor_rec ts W) mpred * mpred * invG) rho =>
     PROPx (map (fun P => P ts _a) (map (fun P ts _a => let '(w, _, _) := _a in P ts w) P)) (LOCALx (map (fun P => P ts _a) (map (fun P ts _a => let '(w, _, _) := _a in P ts w) L))
-     (SEPx (map (fun R => R ts _a) ((fun ts _a => let '(w, Q, inv_names) := _a in atomic_shift(A := A)(inv_names := inv_names) (S2 ts w) Ei Eo (SQ ts w) (fun _ => Q)) ::
+     (SEPx (map (fun R => R ts _a) ((fun ts _a => let '(w, Q, inv_names) := _a in atomic_shift(A := A ts)(inv_names := inv_names) (S2 ts w) Ei Eo (SQ ts w) (fun _ => Q)) ::
         map (fun R ts _a => let '(w, _, _) := _a in R ts w) R)))) rho).
   apply PROP_LOCAL_SEP_super_non_expansive.
   - rewrite Forall_map.
@@ -151,18 +370,10 @@ Proof.
     eapply Forall_impl, HL; simpl; intros.
     intros ?? ((?, ?), ?) ?; simpl; auto.
   - constructor.
-    + intros ?? ((?, ?), ?) ?.
-      unfold atomic_shift; simpl.
-      rewrite !approx_exp; f_equal; extensionality.
-      rewrite -> !approx_sepcon, !approx_andp; f_equal; f_equal.
-      setoid_rewrite fview_shift_nonexpansive; f_equal; f_equal; f_equal.
-      rewrite !approx_exp; f_equal; extensionality.
-      rewrite -> !approx_sepcon, !approx_andp; f_equal; auto.
-      f_equal.
-      * setoid_rewrite fview_shift_nonexpansive; f_equal; f_equal; auto.
-      * rewrite -> !approx_allp by apply tt; f_equal; extensionality.
-        setoid_rewrite fview_shift_nonexpansive; f_equal; f_equal; auto.
-        rewrite approx_idem; auto.
+    + intros ?? ((?, ?), ?) ?; simpl.
+      rewrite -> atomic_shift_nonexpansive; setoid_rewrite atomic_shift_nonexpansive at 2.
+      f_equal; f_equal; repeat extensionality; auto.
+      rewrite approx_idem; auto.
     + rewrite Forall_map.
       eapply Forall_impl, HR; simpl; intros.
       intros ?? ((?, ?), ?) ?; simpl; auto.
@@ -175,7 +386,7 @@ Lemma atomic_spec_nonexpansive_pre : forall {A T} {t : Inhabitant T} W P L R S2 
   (Heq : (forall ts (_a : functors.MixVariantFunctor._functor (dependent_type_functor_rec ts W) mpred * (T -> mpred) * invG),
    Pre ts _a = let '(w, Q, inv_names) := _a in
     PROPx (map (fun P => P ts w) P) (LOCALx (map (fun L => L ts w) L)
-     (SEPx (atomic_shift(A := A)(inv_names := inv_names) (S2 ts w) Ei Eo (SQ ts w) Q :: map (fun R => R ts w) R)))))
+     (SEPx (atomic_shift(A := A ts)(inv_names := inv_names) (S2 ts w) Ei Eo (SQ ts w) Q :: map (fun R => R ts w) R)))))
   (HP : Forall (fun x => super_non_expansive (fun ts w _ => !! (x ts w))) P)
   (HL : Forall (fun x => super_non_expansive (fun ts w rho => !! (locald_denote (x ts w) rho))) L)
   (HR : Forall (fun x => super_non_expansive (fun ts w _ => x ts w)) R),
@@ -289,6 +500,126 @@ Proof.
   rewrite Forall_forall; intro X; apply X; auto.
 Qed.
 
+Definition stable_spec_type W := ProdType (ProdType (ProdType W
+  (ArrowType (DependentType 0) (ArrowType (DependentType 1) Mpred))) (ArrowType (DependentType 1) Mpred)) (ConstType invG).
+
+Lemma stabilize : forall T W args tz P1 P2 Q1 Q2 neP1 neP2 neQ1 neQ2
+  PP la P a lb b Ei Eo Q'
+  (Hpre1 : forall ts w Q inv_names, P1 ts (w, Q, inv_names) =
+     PROP (PP ts w)
+     (LOCALx (map (fun l => l ts w) la)
+     (SEP (atomic_shift(inv_names := inv_names) (a ts w) Ei Eo (b ts w) Q; P ts w))))
+  (Hpost1 : forall ts w Q inv_names, Q1 ts (w, Q, inv_names) =
+     EX v : T, PROP () (LOCALx (map (fun l => l ts w v) lb) (SEP (Q v))))
+  (Hpre2 : forall ts w b' Q inv_names, P2 ts (w, b', Q, inv_names) =
+     PROP (PP ts w)
+     (LOCALx (map (fun l => l ts w) la)
+     (SEP (atomic_shift(inv_names := inv_names) (a ts w) Ei Eo b' Q; P ts w))))
+  (Hpost2 : forall ts w b' Q inv_names, Q2 ts (w, b', Q, inv_names) =
+    EX v1 : _, EX v2 : _,
+     PROP () (LOCALx (map (fun l => l ts w v2) lb)
+     (SEP (atomic_shift(inv_names := inv_names) (a ts w) Ei Eo b' Q; Q' ts w v1 v2))))
+  (Hb : forall ts w v1 v2, b ts w v1 v2 |-- a ts w v1 * Q' ts w v1 v2),
+  funspec_sub (mk_funspec (pair args tz) cc_default (atomic_spec_type W T) P1 Q1 neP1 neQ1)
+    (mk_funspec (pair args tz) cc_default (stable_spec_type W) P2 Q2 neP2 neQ2).
+Proof.
+  intros; apply subsume_subsume.
+  unfold funspec_sub'; repeat (split; auto); intros.
+  destruct x2 as (((w, b'), Q), inv_names).
+  simpl funsig_of_funspec.
+  rewrite Hpre2.
+  set (AS := atomic_shift _ _ _ _ _).
+  Exists ts2 (w, (fun v2 => AS * EX v1 : _, Q' ts2 w v1 v2), inv_names) seplog.emp.
+  simpl in *; intro.
+  unfold liftx; simpl.
+  unfold lift.
+  rewrite emp_sepcon.
+  apply andp_right.
+  - apply andp_left2.
+    rewrite Hpre1.
+    unfold PROPx, LOCALx, SEPx; simpl.
+    do 2 (apply andp_derives; auto).
+    unfold AS, atomic_shift; Intros P'; Exists P'; cancel.
+    sep_apply cored_dup_cored.
+    apply andp_derives; auto.
+    iIntros "[H AS] P"; iMod ("H" with "P") as (v1) "[a H]".
+    iExists v1; iFrame.
+    iIntros "!>"; iSplit.
+    + iIntros "a".
+      iDestruct "AS" as "[_ e]"; iMod (cored_emp with "e") as "_".
+      iApply "H"; auto.
+    + iIntros (y) "b".
+      iDestruct (Hb with "b") as "[a Q]".
+      iMod ("H" with "a").
+      iIntros "!>"; iSplitR "Q".
+      * iExists P'; iFrame.
+      * iExists v1; auto.
+  - apply prop_right; intros.
+    apply andp_left2; rewrite emp_sepcon; auto.
+    rewrite Hpost1 Hpost2.
+    unfold PROPx, LOCALx, SEPx; simpl.
+    Intros v2 v1; Exists v1 v2; rewrite sepcon_assoc; unfold AS; auto.
+Qed.
+
+Lemma stabilize0 : forall W args tz P1 P2 Q1 Q2 neP1 neP2 neQ1 neQ2
+  PP la P a lb b Ei Eo Q'
+  (Hpre1 : forall ts w Q inv_names, P1 ts (w, Q, inv_names) =
+    PROP (PP ts w)
+     (LOCALx (map (fun l => l ts w) la)
+     (SEP (atomic_shift(B := unit)(inv_names := inv_names) (a ts w) Ei Eo (b ts w) (fun _ => Q); P ts w))))
+  (Hpost1 : forall ts w Q inv_names, Q1 ts (w, Q, inv_names) =
+     PROP () (LOCALx (map (fun l => l ts w) lb) (SEP (Q))))
+  (Hpre2 : forall ts w b' Q inv_names, P2 ts (w, b', Q, inv_names) =
+     PROP (PP ts w)
+     (LOCALx (map (fun l => l ts w) la)
+     (SEP (atomic_shift(inv_names := inv_names) (a ts w) Ei Eo b' Q; P ts w))))
+  (Hpost2 : forall ts w b' Q inv_names, Q2 ts (w, b', Q, inv_names) =
+    EX v1 : _,
+     PROP () (LOCALx (map (fun l => l ts w) lb)
+     (SEP (atomic_shift(inv_names := inv_names) (a ts w) Ei Eo b' Q; Q' ts w v1))))
+  (Hb : forall ts w v1, b ts w v1 tt |-- a ts w v1 * Q' ts w v1),
+  funspec_sub (mk_funspec (pair args tz) cc_default (atomic_spec_type0 W) P1 Q1 neP1 neQ1)
+    (mk_funspec (pair args tz) cc_default (stable_spec_type W) P2 Q2 neP2 neQ2).
+Proof.
+  intros; apply subsume_subsume.
+  unfold funspec_sub'; repeat (split; auto); intros.
+  destruct x2 as (((w, b'), Q), inv_names).
+  simpl funsig_of_funspec.
+  rewrite Hpre2.
+  set (AS := atomic_shift _ _ _ _ _).
+  Exists ts2 (w, (AS * EX v1 : _, Q' ts2 w v1), inv_names) seplog.emp.
+  simpl in *; intro.
+  unfold liftx; simpl.
+  unfold lift.
+  rewrite emp_sepcon.
+  apply andp_right.
+  - apply andp_left2.
+    rewrite Hpre1.
+    unfold PROPx, LOCALx, SEPx; simpl.
+    do 2 (apply andp_derives; auto).
+    unfold AS, atomic_shift; Intros P'; Exists P'; cancel.
+    sep_apply cored_dup_cored.
+    apply andp_derives; auto.
+    iIntros "[H AS] P"; iMod ("H" with "P") as (v1) "[a H]".
+    iExists v1; iFrame.
+    iIntros "!>"; iSplit.
+    + iIntros "a".
+      iDestruct "AS" as "[_ e]"; iMod (cored_emp with "e") as "_".
+      iApply "H"; auto.
+    + iIntros ([]) "b".
+      iDestruct (Hb with "b") as "[a Q]".
+      iMod ("H" with "a").
+      iIntros "!>"; iSplitR "Q".
+      * iExists P'; iFrame.
+      * iExists v1; auto.
+  - apply prop_right; intros.
+    apply andp_left2; rewrite emp_sepcon; auto.
+    rewrite Hpost1 Hpost2.
+    unfold PROPx, LOCALx, SEPx; simpl.
+    Intros v1; Exists v1; rewrite sepcon_assoc; unfold AS; auto.
+Qed.
+
+
 Notation "'ATOMIC' 'TYPE' W 'OBJ' x 'INVS' Ei Eo 'WITH' x1 : t1 'PRE'  [ u , .. , v ] 'PROP' ( Px ; .. ; Py ) 'LOCAL' ( Lx ; .. ; Ly ) 'SEPS' ( S1x ; .. ; S1y ) '|' S2 'POST' [ tz ] 'EX' r : T , 'PROP' () 'LOCAL' ( LQx ; .. ; LQy ) 'SEP' ( SQx ; .. ; SQy )" :=
   (mk_funspec (pair (cons u%formals .. (cons v%formals nil) ..) tz) cc_default (atomic_spec_type W T)
    (fun (ts: list Type) (__a : functors.MixVariantFunctor._functor (dependent_type_functor_rec ts W) mpred * (T -> mpred) * invG) => let '(x1, Q, inv_names) := __a in
@@ -304,8 +635,7 @@ Notation "'ATOMIC' 'TYPE' W 'OBJ' x 'INVS' Ei Eo 'WITH' x1 : t1 'PRE'  [ u , .. 
       (fun ts __a x => let x1 := __a in S2) Ei Eo
      (fun ts __a x r => let x1 := __a in fold_right_sepcon (cons SQx%logic .. (cons SQy%logic nil) ..)) _ _ _ _ _)
    (atomic_spec_nonexpansive_post' W (cons (fun ts __a r => let x1 := __a in LQx%logic) .. (cons (fun ts __a r => let x1 := __a in LQy%logic) nil) ..) _)) (at level 200, x at level 0, Ei at level 0, Eo at level 0, x1 at level 0,
-        x1 at level 0,
-             S2 at level 0, r at level 0, T at level 0).
+        x1 at level 0, S2 at level 0, r at level 0, T at level 0).
 
 Notation "'ATOMIC' 'TYPE' W 'OBJ' x 'INVS' Ei Eo 'WITH' x1 : t1 'PRE'  [ u , .. , v ] 'PROP' ( Px ; .. ; Py ) 'LOCAL' ( Lx ; .. ; Ly ) 'SEPS' ( S1x ; .. ; S1y ) '|' S2 'POST' [ tz ] 'EX' r : T , 'PROP' () 'LOCAL' ( LQx ; .. ; LQy ) 'SEP' ( SQx ; .. ; SQy )" :=
   (mk_funspec (pair (cons u%formals .. (cons v%formals nil) ..) tz) cc_default (atomic_spec_type W T)
@@ -789,7 +1119,8 @@ Notation "'ATOMIC' 'TYPE' W 'OBJ' x 'INVS' Ei Eo 'WITH' x1 : t1 , x2 : t2 , x3 :
         x1 at level 0, x2 at level 0, x3 at level 0, x4 at level 0, x5 at level 0, x6 at level 0, x7 at level 0, x8 at level 0, x9 at level 0,
              S2 at level 0, r at level 0, T at level 0).
 
-Global Obligation Tactic := repeat constructor || let x := fresh "x" in intros ?? x; repeat destruct x as [x ?]; reflexivity.
+
+Global Obligation Tactic := repeat constructor || let x := fresh "x" in intros ?? x; repeat destruct x as [x ?]; simpl; auto.
 
 Ltac start_atomic_function :=
 (*  match goal with |- semax_body ?V ?G ?F ?spec =>
