atomics/general_locks.v
@@ -12,6 +12,7 @@ Section locks.
 Context {CS : compspecs}.
 
 Parameters (locked unlocked : val -> mpred). (* instantiation depends on the lock implementation *)
+Axioms (locked_timeless : forall p, Timeless (locked p)) (unlocked_timeless : forall p, Timeless (unlocked p)).
 
 Definition makelock_spec :=
   WITH p : val
@@ -60,24 +61,50 @@ Program Definition release_spec :=
     SEP (unlocked p).
 
 
-Definition lock_inv' {A : Type} lock g (a : A) R := (unlocked lock * ghost_part_ref(P := discrete_PCM A) g Tsh a a * |>R a) ||
+Definition lock_inv' {A : Type} lock g (a : A) R := (unlocked lock * ghost_part_ref(P := discrete_PCM A) g Tsh a a * R a) ||
   (locked lock * ghost_part(P := discrete_PCM A) g Tsh a).
+
+Global Instance lock_inv'_timeless {A} lock g (a : A) R (HR : forall a, Timeless (R a)): Timeless (lock_inv' lock g a R).
+Proof.
+  unfold lock_inv'.
+  apply (@bi.or_timeless mpredSI).
+  - apply (@bi.sep_timeless mpredSI); auto.
+    apply (@bi.sep_timeless mpredSI); [apply unlocked_timeless | apply _].
+  - apply (@bi.sep_timeless mpredSI); [apply locked_timeless | apply _].
+Qed.
 
 Lemma lock_inv'_nonexpansive : forall {A} n x g x0 _f,
   approx n (lock_inv' x g x0 _f) = approx n (lock_inv' x g x0 (λ a : A, approx n (_f a))).
 Proof.
   intros; unfold lock_inv'.
-  rewrite !approx_orp !approx_sepcon; f_equal; f_equal.
-  destruct n; [rewrite !approx_0; auto|].
-  rewrite !approx_later; f_equal.
-  change (approx n (approx (S n) (_f x0))) with ((approx n oo approx (S n)) (_f x0)).
-  rewrite -> approx_oo_approx'; auto.
+  rewrite !approx_orp !approx_sepcon approx_idem; auto.
 Qed.
 
-(* can we make A a dependent type argument? *)
-Program Definition acquire_spec' {A : Type} :=
-  ATOMIC TYPE (ProdType (ConstType (_ * _)) (ArrowType (ConstType A) Mpred)) OBJ a INVS empty top
-  WITH p : val, g : gname, R : A -> mpred
+Definition timeless_inv {A} R : mpred := ALL a : A, |> R a -* sbi_except_0 (R a).
+
+Lemma timeless_inv_nonexpansive: forall {A} n (R : A -> mpred),
+  approx n (timeless_inv R) = approx n (timeless_inv (fun a => approx n (R a))).
+Proof.
+  intros; unfold timeless_inv.
+  rewrite allp_nonexpansive; setoid_rewrite allp_nonexpansive at 2; f_equal; f_equal; extensionality.
+  rewrite wand_nonexpansive; setoid_rewrite wand_nonexpansive at 2; f_equal; f_equal.
+  - apply later_nonexpansive.
+  - unfold sbi_except_0.
+    rewrite !approx_orp approx_idem; auto.
+Qed.
+
+Lemma timeless_inv_timeless : forall {A} (R : A -> mpred) {H : forall a, Timeless (R a)},
+  seplog.emp |-- timeless_inv R && seplog.emp.
+Proof.
+  intros; apply andp_right; auto.
+  intros; unfold timeless_inv.
+  iIntros "_" (a) "R".
+  iApply (timeless with "R").
+Qed.
+
+Program Definition acquire_spec' :=
+  ATOMIC TYPE (ProdType (ConstType (_ * _)) (ArrowType (DependentType 0) Mpred)) OBJ a INVS empty top
+  WITH p : val, g : gname, R : _
   PRE [ 1%positive OF tptr tvoid ]
     PROP (True)
     LOCAL (temp 1%positive p)
@@ -85,37 +112,18 @@ Program Definition acquire_spec' {A : Type} :=
   POST [ tvoid ]
     PROP ()
     LOCAL ()
-    SEP (lock_inv' p g a R; ghost_reference(P := discrete_PCM A) g a; |>R a).
+    SEP (lock_inv' p g a R; ghost_reference(P := discrete_PCM _) g a; R a).
 Next Obligation.
-  let x := fresh "x" in intros ??? x; repeat destruct x as [x ?]; simpl; intros.
+  intros; apply lock_inv'_nonexpansive.
+Qed.
+Next Obligation.
+  intros; rewrite !approx_sepcon approx_idem; f_equal.
   apply lock_inv'_nonexpansive.
 Qed.
-Next Obligation.
-  let x := fresh "x" in intros ??? x; repeat destruct x as [x ?]; simpl; intros.
-  rewrite !approx_sepcon; f_equal.
-  - apply lock_inv'_nonexpansive.
-  - f_equal; f_equal.
-    destruct n; [rewrite !approx_0; auto|].
-    rewrite !approx_later; f_equal.
-   change (approx n (approx (S n) (_f x0))) with ((approx n oo approx (S n)) (_f x0)).
-    rewrite -> approx_oo_approx'; auto.
-Qed.
-Next Obligation.
-  let x := fresh "x" in intros ??? x; repeat destruct x as [x ?]; simpl; intros; auto.
-Qed.
-Next Obligation.
-  let x := fresh "x" in intros ??? x; repeat destruct x as [x ?]; simpl; intros; auto.
-Qed.
-Next Obligation.
-  let x := fresh "x" in intros ??? x; repeat destruct x as [x ?]; simpl; intros; auto.
-Qed.
-Next Obligation.
-  let x := fresh "x" in intros ??? x; repeat destruct x as [x ?]; simpl; intros; auto.
-Qed.
 
-Lemma acquire_sub : forall {A : Type}, funspec_sub acquire_spec (@acquire_spec' A).
+Lemma acquire_sub : funspec_sub acquire_spec acquire_spec'.
 Proof.
-  intro; apply subsume_subsume.
+  apply subsume_subsume.
   unfold funspec_sub', acquire_spec, acquire_spec'; intros; repeat (split; auto); intros.
   destruct x2 as ((((p, g), R), Q), inv_names).
   simpl funsig_of_funspec.
@@ -128,74 +136,53 @@ Proof.
   - apply andp_left2.
     unfold PROPx, LOCALx, SEPx; simpl; entailer!.
     apply andp_derives; auto.
-    unfold atomic_shift.
-    Intros P; Exists P; cancel.
-    apply andp_derives; auto.
-    apply wand_derives; auto.
-    iIntros ">H !>".
-    iDestruct "H" as (a) "[lock Hclose]".
+    apply atomic_shift_derives'; intros.
+    iIntros "lock !>".
     unfold lock_inv' at 1; iDestruct "lock" as "[[[u a] R] | [l a]]".
     + iExists true; iSplitL "u"; first by iRight; iFrame.
       iSplit.
-      * iIntros "[[% ?] | [% ?]]"; try discriminate.
-        iApply "Hclose".
+      * iIntros "[[% ?] | [% ?]] !>"; try discriminate.
         unfold lock_inv'; iLeft; iFrame.
-      * iIntros (_) "[[_ l] _]".
-        iDestruct "Hclose" as "[_ Hclose]"; iApply ("Hclose" $! tt).
+      * iIntros (_) "[[_ l] _] !>".
         rewrite <- ghost_part_ref_join; iDestruct "a" as "[? ?]"; iFrame.
         unfold lock_inv'; iRight; iFrame.
     + iExists false; iSplitL "l"; first by iLeft; iFrame.
       iSplit.
-      * iIntros "[[% ?] | [% ?]]"; try discriminate.
-        iApply "Hclose".
+      * iIntros "[[% ?] | [% ?]] !>"; try discriminate.
         unfold lock_inv'; iRight; iFrame.
       * iIntros (_) "[[% l] _]"; discriminate.
   - apply prop_right; intros.
     apply andp_left2; rewrite emp_sepcon; auto.
 Qed.
 
-Program Definition release_spec' {A : Type} :=
-  ATOMIC TYPE (ProdType (ConstType (_ * _ * _ * _)) (ArrowType (ConstType A) Mpred)) OBJ a INVS empty top
-  WITH p : val, g : gname, b : A, b' : A, R : A -> mpred
+Definition release_type' := (ProdType (ProdType (ProdType (ConstType (val * gname))
+  (DependentType 0)) (DependentType 0)) (ArrowType (DependentType 0) Mpred)).
+
+Program Definition release_spec' :=
+  ATOMIC TYPE release_type' OBJ a INVS empty top
+  WITH p : val, g : gname, b : _, b' : _, R : _ -> mpred
   PRE [ 1%positive OF tptr tvoid ]
     PROP (True)
     LOCAL (temp 1%positive p)
-    SEPS (ghost_reference(P := discrete_PCM A) g b; |>R b') | (lock_inv' p g a R)
+    SEPS (timeless_inv R && seplog.emp; ghost_reference(P := discrete_PCM _) g b; |>R b') | (lock_inv' p g a R)
   POST [ tvoid ]
     PROP ()
     LOCAL ()
     SEP (!!(a = b) && lock_inv' p g b' R).
 Next Obligation.
-  let x := fresh "x" in intros ?? x; repeat destruct x as [x ?]; simpl; intros.
-  destruct n; [rewrite !approx_0; auto|].
-  rewrite !approx_later; f_equal.
-  change (approx n (approx (S n) (_f a))) with ((approx n oo approx (S n)) (_f a)).
-  rewrite -> approx_oo_approx'; auto.
+  intros; rewrite !approx_andp timeless_inv_nonexpansive; auto.
+  intros; rewrite later_nonexpansive; auto.
 Qed.
 Next Obligation.
-  let x := fresh "x" in intros ??? x; repeat destruct x as [x ?]; simpl; intros.
-  rewrite lock_inv'_nonexpansive; auto.
+  intros; rewrite lock_inv'_nonexpansive; auto.
 Qed.
 Next Obligation.
-  let x := fresh "x" in intros ??? x; repeat destruct x as [x ?]; simpl; intros; auto.
-  rewrite !sepcon_emp !approx_andp lock_inv'_nonexpansive; auto.
-Qed.
-Next Obligation.
-  let x := fresh "x" in intros ??? x; repeat destruct x as [x ?]; simpl; intros; auto.
-  Qed.
-Next Obligation.
-  let x := fresh "x" in intros ??? x; repeat destruct x as [x ?]; simpl; intros; auto.
-Qed.
-Next Obligation.
-  let x := fresh "x" in intros ??? x; repeat destruct x as [x ?]; simpl; intros; auto.
-Qed.
-Next Obligation.
-  let x := fresh "x" in intros ??? x; repeat destruct x as [x ?]; simpl; intros; auto.
+  intros; rewrite !sepcon_emp !approx_andp lock_inv'_nonexpansive; auto.
 Qed.
 
-Lemma release_sub : forall {A : Type}, funspec_sub release_spec (@release_spec' A).
+Lemma release_sub : funspec_sub release_spec release_spec'.
 Proof.
-  intro; apply subsume_subsume.
+  apply subsume_subsume.
   unfold funspec_sub', release_spec, release_spec'; intros; repeat (split; auto); intros.
   destruct x2 as ((((((p, g), b), b'), R), Q), inv_names).
   simpl funsig_of_funspec.
@@ -208,16 +195,14 @@ Proof.
   - apply andp_left2.
     unfold PROPx, LOCALx, SEPx; simpl; entailer!.
     apply andp_derives; auto.
-    unfold atomic_shift.
-    Intros P; Exists (P * ghost_reference(P := discrete_PCM A) g b * R b').
-    rewrite !later_sepcon; cancel.
-    apply andp_derives; auto.
-    iIntros "H [[P >b] R]".
-    iMod ("H" with "P") as (a) "[lock Hclose]"; subst.
-    iIntros "!>"; iExists tt.
+    rewrite sepcon_assoc; eapply derives_trans, atomic_shift_derives_frame_cored.
+    { apply sepcon_derives; [apply derives_refl|].
+      setoid_rewrite later_sepcon; apply sepcon_derives; [apply now_later | apply derives_refl]. }
+    { apply andp_left2, emp_cored. }
+    iIntros (a) "[[lock timeless] [>b R]] !>"; iExists tt.
     unfold lock_inv' at 1; iDestruct "lock" as "[[[u a'] R'] | [l a]]".
     + iCombine "b a'" as "a".
-      iPoseProof (own_valid_2(RA := ref_PCM (discrete_PCM A)) with "a") as "%".
+      iPoseProof (own_valid_2(RA := ref_PCM (discrete_PCM _)) with "a") as "%".
       hnf in H.
       destruct H as ((?, ?) & J & _).
       inv J; simpl in *.
@@ -225,20 +210,159 @@ Proof.
       inv H3.
     + iFrame; iSplit.
       * iIntros "l".
-        iMod ("Hclose" with "[l a]").
-        { iFrame; unfold lock_inv'; iRight; iFrame. }
-        iFrame; auto.
+        iFrame; iSplitR "timeless"; auto.
+        unfold lock_inv'; iRight; iFrame; auto.
       * iIntros (_) "u".
         iCombine "a b" as "a".
-        iPoseProof (ref_sub(P := discrete_PCM A) with "a") as "%".
+        iPoseProof (ref_sub(P := discrete_PCM _) with "a") as "%".
         rewrite eq_dec_refl in H; subst.
         setoid_rewrite ghost_part_ref_join.
-        iMod (ref_update(P := discrete_PCM A) with "a").
-        iDestruct "Hclose" as "[_ Hclose]"; iApply ("Hclose" $! tt).
+        iMod (ref_update(P := discrete_PCM _) with "a").
+        unfold timeless_inv.
+        iMod ("timeless" with "R").
+        iIntros "!>"; iExists tt; iFrame.
+        iSplitR ""; [|by iIntros "?"].
         iSplit; auto; iSplit; auto.
         unfold lock_inv'; iLeft; iFrame.
   - apply prop_right; intros.
     apply andp_left2; rewrite emp_sepcon; auto.
+Qed.
+
+Definition acq_type := ProdType (ProdType (ProdType (ProdType (ConstType (val * gname))
+  (ArrowType (DependentType 0) Mpred)) (ArrowType (DependentType 0) (ArrowType (DependentType 1) Mpred)))
+  (ArrowType (DependentType 1) Mpred)) (ConstType invG).
+
+Program Definition acquire_inv_spec :=
+  TYPE acq_type WITH p : val, g : gname, R : _ -> mpred, b : _, Q : _, inv_names : invG
+  PRE [ 1%positive OF tptr tvoid ]
+    PROP (True)
+    LOCAL (temp 1%positive p)
+    SEP (atomic_shift (fun a => lock_inv' p g a R) empty top b Q)
+  POST [ tvoid ]
+   EX a : _,
+    PROP ()
+    LOCAL ()
+    SEP (atomic_shift (fun a => lock_inv' p g a R) empty top b Q;
+            ghost_reference(P := discrete_PCM _) g a; R a).
+Next Obligation.
+Proof.
+  intros; unfold PROPx, LOCALx, SEPx; simpl; rewrite !approx_andp; f_equal;
+    f_equal; rewrite -> !sepcon_emp, ?approx_sepcon, ?approx_idem.
+  rewrite atomic_shift_nonexpansive; setoid_rewrite atomic_shift_nonexpansive at 2.
+  f_equal; f_equal; repeat extensionality; rewrite ?approx_idem; auto.
+  apply lock_inv'_nonexpansive.
+Qed.
+Next Obligation.
+Proof.
+  intros; rewrite !approx_exp; apply f_equal; extensionality.
+  unfold PROPx, LOCALx, SEPx; simpl; rewrite !approx_andp; do 2 apply f_equal;
+    rewrite -> !sepcon_emp, ?approx_sepcon, ?approx_idem; auto.
+  f_equal.
+  rewrite atomic_shift_nonexpansive; setoid_rewrite atomic_shift_nonexpansive at 2.
+  f_equal; f_equal; repeat extensionality; rewrite ?approx_idem; auto.
+  apply lock_inv'_nonexpansive.
+Qed.
+
+Lemma acquire_inv : funspec_sub acquire_spec acquire_inv_spec.
+Proof.
+  eapply funspec_sub_trans; [apply acquire_sub|].
+  eapply stabilize0; intros ? ((?, ?), ?); intros; simpl.
+  - apply f_equal2.
+    { instantiate (1 := fun _ _ => _); auto. }
+    apply f_equal2.
+    { instantiate (1 := [fun _ '(p, _, _) => temp _ p]); auto. }
+    unfold SEPx; simpl; extensionality; apply f_equal2.
+    { instantiate (1 := fun ts '(p, g, R) a _ => _).
+      instantiate (4 := fun ts '(p, g, R) a => _); auto. }
+    { instantiate (1 := fun _ _ => seplog.emp); auto. }
+  - instantiate (1 := nil); auto.
+  - f_equal; f_equal.
+    unfold SEPx; simpl.
+    rewrite !sepcon_emp; auto.
+  - extensionality; simpl.
+    apply f_equal; extensionality.
+    unfold PROPx, LOCALx, SEPx; simpl.
+    apply f_equal2; [auto|].
+    apply f_equal2; [auto|].
+    rewrite !sepcon_emp.
+    instantiate (1 := fun _ '(p, g, R) a => _); auto.
+  - simpl.
+    rewrite sepcon_emp; apply derives_refl.
+Qed.
+
+Definition rel_type := ProdType (ProdType (ProdType (ProdType (ProdType (ConstType (val * gname))
+   (DependentType 0)) (ArrowType (DependentType 0) Mpred)) (ArrowType (DependentType 0) (ArrowType (DependentType 1) Mpred)))
+  (ArrowType (DependentType 1) Mpred)) (ConstType invG).
+
+(* This version of release only works if the invariant has been re-established; otherwise,
+  you need to use release_spec' and show that you've reached your linearization point. *)
+Program Definition release_inv_spec :=
+  TYPE rel_type WITH p : val, g : gname, a : _, R : _ -> mpred, b : _ -> _ -> mpred, Q : _ -> mpred, inv_names : invG
+  PRE [ 1%positive OF tptr tvoid ]
+    PROP (True)
+    LOCAL (temp 1%positive p)
+    SEP (timeless_inv R && seplog.emp; atomic_shift (fun a => lock_inv' p g a R) empty top b Q;
+            ghost_reference(P := discrete_PCM _) g a; R a)
+  POST [ tvoid ]
+    PROP ()
+    LOCAL ()
+    SEP (atomic_shift (fun a => lock_inv' p g a R) empty top b Q).
+Next Obligation.
+Proof.
+  intros; unfold PROPx, LOCALx, SEPx; simpl; rewrite !approx_andp; f_equal;
+    f_equal; rewrite -> !sepcon_emp, ?approx_sepcon, ?approx_idem.
+  f_equal.
+  { rewrite !approx_andp timeless_inv_nonexpansive; auto. }
+  f_equal.
+  rewrite atomic_shift_nonexpansive; setoid_rewrite atomic_shift_nonexpansive at 2.
+  f_equal; f_equal; repeat extensionality; rewrite ?approx_idem; auto.
+  apply lock_inv'_nonexpansive.
+Qed.
+Next Obligation.
+Proof.
+  intros.
+  unfold PROPx, LOCALx, SEPx; simpl; rewrite !approx_andp; do 2 apply f_equal;
+    rewrite -> !sepcon_emp, ?approx_sepcon, ?approx_idem; auto.
+  rewrite atomic_shift_nonexpansive; setoid_rewrite atomic_shift_nonexpansive at 2.
+  f_equal; f_equal; repeat extensionality; rewrite ?approx_idem; auto.
+  apply lock_inv'_nonexpansive.
+Qed.
+
+(* Because of this distinction, it's a bit awkward to phrase this as a stabilization. *)
+Lemma release_inv : funspec_sub release_spec release_inv_spec.
+Proof.
+  eapply funspec_sub_trans; [apply release_sub|].
+  apply subsume_subsume; unfold funspec_sub', release_spec', release_inv_spec.
+  repeat split; auto; intros.
+  destruct x2 as ((((((p, g), a), R), b), Q), inv_names).
+  simpl funsig_of_funspec.
+  set (AS := atomic_shift _ _ _ _ _).
+  unfold AS, atomic_shift; Intros P.
+  Exists ts2 (p, g, a, a, R, AS, inv_names) seplog.emp.
+  simpl; intro.
+  unfold liftx; simpl.
+  unfold lift.
+  rewrite emp_sepcon.
+  apply andp_right.
+  - apply andp_left2.
+    unfold PROPx, LOCALx, SEPx; simpl; entailer!.
+    Exists P.
+    apply andp_derives; auto.
+    cancel.
+    sep_apply cored_dup_cored.
+    apply andp_derives; auto.
+    unfold ashift at 1 3.
+    iIntros "[H AS] P"; iMod ("H" with "P") as (a') "[lock H]".
+    iExists a'; iFrame.
+    iIntros "!>"; iSplit.
+    + iDestruct "AS" as "[_ e]"; iMod (cored_emp with "e") as "_".
+      by iApply bi.and_elim_l.
+    + iIntros (_) "[[% lock] _]"; subst.
+      iMod ("H" with "lock").
+      unfold AS, atomic_shift; iExists P; iFrame; auto.
+  - apply prop_right; intros.
+    apply andp_left2; rewrite emp_sepcon.
+    apply derives_refl.
 Qed.
 
 End locks.
